tuning file structure
Renaming:
* CDCL_Two_Watched_Literals_IsaSAT ~> IsaSAT
* CDCL_Two_Watched_Literals ~> Two_Watched_Literals

Deletion:
* CDCL_Two_Watched_Literals_Watch_List_Code_Common'

Weidenbach_Book/Two_Watched_Literals_Watch_List_Code_Common.thy
@@ -1,7 +1,174 @@
-theory CDCL_Two_Watched_Literals_Watch_List_Code_Common
-  imports CDCL_Two_Watched_Literals_Code_Common CDCL_Two_Watched_Literals_Watch_List_Domain
+theory Two_Watched_Literals_Watch_List_Code_Common
+  imports Two_Watched_Literals_Watch_List_Domain
     Bits_Natural WB_Word_Assn
 begin
+text \<open>
+  First we instantiate our types with sort heap and default, to have compatibility with code
+  generation. The idea is simplify to create injections into the components of our datatypes.
+\<close>
+instance literal :: (heap) heap
+proof standard
+  obtain f :: \<open>'a \<Rightarrow> nat\<close> where f: \<open>inj f\<close>
+    by blast
+  then have Hf: \<open>f x = f s \<longleftrightarrow> x = s\<close> for s x
+    unfolding inj_on_def Ball_def comp_def by blast
+  let ?f = \<open>\<lambda>L. (is_pos L, f (atm_of L))\<close>
+  have \<open>OFCLASS(bool \<times> nat, heap_class)\<close>
+   by standard
+  then obtain g :: \<open>bool \<times> nat \<Rightarrow> nat\<close> where g: \<open>inj g\<close>
+    by blast
+  then have H: \<open>g (x, y) = g (s, t) \<longleftrightarrow> x = s \<and> y = t\<close> for s t x y
+    unfolding inj_on_def Ball_def comp_def by blast
+  have \<open>inj (g o ?f)\<close>
+    using f g unfolding inj_on_def Ball_def comp_def H Hf
+    apply (intro allI impI)
+    apply (rename_tac x y, case_tac x; case_tac y)
+    by auto
+  then show \<open>\<exists>to_nat:: 'a literal \<Rightarrow> nat. inj to_nat\<close>
+    by blast
+qed
+
+instance annotated_lit :: (heap, heap, heap) heap
+proof standard
+  let ?f = \<open>\<lambda>L:: ('a, 'b, 'c) annotated_lit.
+      (if is_decided L then Some (lit_dec L) else None,
+       if is_decided L then None else Some (lit_prop L), if is_decided L then None else Some (mark_of L))\<close>
+  have f: \<open>inj ?f\<close>
+    unfolding inj_on_def Ball_def
+    apply (intro allI impI)
+    apply (rename_tac x y, case_tac x; case_tac y)
+    by auto
+  then have Hf: \<open>?f x = ?f s \<longleftrightarrow> x = s\<close> for s x
+    unfolding inj_on_def Ball_def comp_def by blast
+  have \<open>OFCLASS('a option \<times> 'b option \<times> 'c option, heap_class)\<close>
+   by standard
+  then obtain g :: \<open>'a option \<times> 'b option \<times> 'c option \<Rightarrow> nat\<close> where g: \<open>inj g\<close>
+    by blast
+  then have H: \<open>g (x, y) = g (s, t) \<longleftrightarrow> x = s \<and> y = t\<close> for s t x y
+    unfolding inj_on_def Ball_def comp_def by blast
+  have \<open>inj (g o ?f)\<close>
+    using f g unfolding inj_on_def Ball_def comp_def H Hf
+    apply (intro allI impI)
+    apply (rename_tac x y, case_tac x; case_tac y)
+    by auto
+  then show \<open>\<exists>to_nat:: ('a, 'b, 'c) annotated_lit \<Rightarrow> nat. inj to_nat\<close>
+    by blast
+qed
+
+instantiation literal :: (default) default
+begin
+definition default_literal where
+\<open>default_literal = Pos default\<close>
+instance by standard
+end
+
+
+subsection \<open>Declaration of some Operators and Implementation\<close>
+
+sepref_decl_op atm_of: "atm_of :: nat literal \<Rightarrow> nat" ::
+  "(Id :: (nat literal \<times> _) set) \<rightarrow> (Id :: (nat \<times> _) set)" .
+
+lemma [def_pat_rules]:
+  "atm_of \<equiv> op_atm_of"
+  by auto
+
+sepref_decl_op lit_of: "lit_of :: (nat, nat) ann_lit \<Rightarrow> nat literal" ::
+  "(Id :: ((nat, nat) ann_lit \<times> _) set) \<rightarrow> (Id :: (nat literal \<times> _) set)" .
+
+lemma [def_pat_rules]:
+  "lit_of \<equiv> op_lit_of"
+  by auto
+
+
+section \<open>Code for the initialisation of the Data Structure\<close>
+
+definition init_dt_step_l :: \<open>'v clause_l \<Rightarrow> 'v twl_st_l_init \<Rightarrow> ('v twl_st_l_init) nres\<close> where
+  \<open>init_dt_step_l C S = do {
+   (let ((M, N, U, D, NP, UP, WS, Q), OC) = S in
+   (case D of
+      None \<Rightarrow>
+        if length C = 0
+        then RETURN ((M, N, U, Some {#}, NP, UP, {#}, {#}), add_mset {#} OC)
+        else if length C = 1
+        then do {
+          ASSERT (no_dup M);
+          ASSERT (C \<noteq> []);
+          let L = hd C;
+          let val_L = polarity M L;
+          if val_L = None
+          then RETURN ((Propagated L 0 # M, N, U, None, add_mset {#L#} NP, UP, WS, add_mset (-L) Q),
+             OC)
+          else
+            if val_L = Some True
+            then RETURN ((M, N, U, None, add_mset {#L#} NP, UP, WS, Q), OC)
+            else RETURN ((M, N, U, Some (mset C), add_mset {#L#} NP, UP, {#}, {#}), OC)
+          }
+        else do {
+          ASSERT(C \<noteq> []);
+          ASSERT(tl C \<noteq> []);
+          RETURN ((M, N @ [C], length N, None, NP, UP, WS, Q), OC)}
+  | Some D \<Rightarrow>
+      RETURN ((M, N, U, Some D, NP, UP, WS, Q), add_mset (mset C) OC)))
+  }\<close>
+
+lemma length_ge_Suc_0_tl_not_nil: \<open>length C > Suc 0 \<Longrightarrow> tl C \<noteq> []\<close>
+  by (cases C) auto
+
+lemma init_dt_step_init_dt_step_l:
+  assumes
+    struct_invs: \<open>twl_struct_invs_init (twl_st_of_init S)\<close>
+  shows \<open>RETURN (init_dt_step C S) = init_dt_step_l C S\<close>
+proof -
+  have \<open>no_dup (trail (state\<^sub>W_of_init (twl_st_of_init S)))\<close>
+    using struct_invs unfolding twl_struct_invs_init_def cdcl\<^sub>W_restart_mset.cdcl\<^sub>W_all_struct_inv_def
+      cdcl\<^sub>W_restart_mset.cdcl\<^sub>W_M_level_inv_def twl_st_of_init.simps
+      by fast
+  then have n_d: \<open>no_dup (get_trail_l (fst S))\<close>
+    by (cases S) (auto simp add: cdcl\<^sub>W_restart_mset_state)
+
+  show ?thesis
+    using n_d  unfolding init_dt_step_def init_dt_step_l_def Let_def
+    by (cases S; cases C; cases \<open>tl C\<close>)
+      (auto simp: polarity_def length_ge_Suc_0_tl_not_nil split: option.splits cong: bind_cong)
+qed
+
+
+definition init_dt_l where
+  \<open>init_dt_l CS S = nfoldli CS (\<lambda>_. True) init_dt_step_l S\<close>
+
+
+lemma init_dt_init_dt_l:
+  assumes
+    \<open>\<forall>C \<in> set CS. distinct C\<close> and
+    \<open>twl_struct_invs_init (twl_st_of_init S)\<close> and
+    \<open>clauses_to_update_l (fst S) = {#}\<close> and
+    \<open>\<forall>s\<in>set (get_trail_l (fst S)). \<not>is_decided s\<close> and
+    \<open>get_conflict_l (fst S) = None \<longrightarrow>
+        literals_to_update_l (fst S) = uminus `# lit_of `# mset (get_trail_l (fst S))\<close> and
+    \<open>additional_WS_invs (fst S)\<close> and
+    \<open>get_learned_l (fst S) = length (get_clauses_l (fst S)) - 1\<close> and
+    \<open>twl_stgy_invs (twl_st_of None (fst S))\<close> and
+    \<open>snd S \<noteq> {#} \<longrightarrow> get_conflict_l (fst S) \<noteq> None\<close>
+  shows \<open>RETURN (init_dt CS S) = init_dt_l (rev CS) S\<close>
+  using assms unfolding init_dt_l_def
+proof (induction CS)
+  case Nil
+  then show ?case by simp
+next
+  case (Cons a CS)
+  then have IH: \<open>RETURN (init_dt CS S) = nfoldli (rev CS) (\<lambda>_. True) init_dt_step_l S\<close>
+    by auto
+  have [simp]: \<open>nfoldli [] (\<lambda>_. True) init_dt_step_l = (\<lambda>S. RETURN S)\<close>
+    by (auto intro!: ext)
+  have step:
+    \<open>RETURN (init_dt_step a (init_dt CS S)) = init_dt_step_l a (init_dt CS S)\<close>
+    apply (rule init_dt_step_init_dt_step_l)
+    subgoal by (rule init_dt_full[of CS \<open>fst S\<close> \<open>snd S\<close>, unfolded prod.collapse])
+        (use Cons(2-) in \<open>solves simp\<close>)+
+    done
+  show ?case
+    by (auto simp: IH[symmetric] step)
+qed
 
 lemma \<open>(return o (\<lambda>n. shiftr n 1), RETURN o shiftr1) \<in> word_nat_assn\<^sup>k \<rightarrow>\<^sub>a word_nat_assn\<close>
   by sepref_to_hoare (sep_auto simp: shiftr1_def word_nat_rel_def unat_shiftr br_def)
